zero padded nacl

code/api/Hacl.Box.ZeroPad.fst
@@ -1,73 +1,36 @@
-module NaCl
+module Hacl.Box.ZeroPad
 
 open FStar.Buffer
 open FStar.ST
-open Hacl.Constants
-open Hacl.Policies
 open Hacl.Cast
 
+open Hacl.Constants
+open Hacl.SecretBox.ZeroPad
+
+
+(* Module abbreviations *)
 module HS  = FStar.HyperStack
 module B   = FStar.Buffer
 module U8  = FStar.UInt8
 module U32 = FStar.UInt32
 module U64 = FStar.UInt64
 
-let crypto_box_NONCEBYTES     = 24
-let crypto_box_PUBLICKEYBYTES = 32
-let crypto_box_SECRETKEYBYTES = 32
-let crypto_box_MACBYTES       = 16
 
-let crypto_secretbox_NONCEBYTES = 24
-let crypto_secretbox_KEYBYTES   = 32
-let crypto_secretbox_MACBYTES   = 16
+#reset-options "--initial_fuel 0 --max_fuel 0 --z3rlimit 5"
 
-val crypto_secretbox_detached:
-  c:uint8_p ->
-  mac:uint8_p{length mac = crypto_secretbox_MACBYTES /\ disjoint mac c} ->
-  m:uint8_p ->
-  mlen:u64{let len = U64.v mlen in len = length m /\ len = length c}  ->
-  n:uint8_p{length n = crypto_secretbox_NONCEBYTES} ->
-  k:uint8_p{length k = crypto_secretbox_KEYBYTES} ->
-  Stack u32
-    (requires (fun h -> live h c /\ live h mac /\ live h m /\ live h n /\ live h k))
-    (ensures  (fun h0 z h1 -> modifies_2 c mac h0 h1 /\ live h1 c /\ live h1 mac))
-let crypto_secretbox_detached c mac m mlen n k = Hacl.SecretBox.ZeroPad.crypto_secretbox_detached c mac m mlen n k
+private val lemma_max_uint32: n:nat -> Lemma
+  (requires (n = 32))
+  (ensures  (pow2 n = 4294967296))
+  [SMTPat (pow2 n)]
+let lemma_max_uint32 n = assert_norm(pow2 32 = 4294967296)
+private val lemma_max_uint64: n:nat -> Lemma
+  (requires (n = 64))
+  (ensures  (pow2 n = 18446744073709551616))
+  [SMTPat (pow2 n)]
+let lemma_max_uint64 n = assert_norm(pow2 64 = 18446744073709551616)
 
-val crypto_secretbox_open_detached:
-  m:uint8_p ->
-  c:uint8_p ->
-  mac:uint8_p{length mac = crypto_secretbox_MACBYTES /\ declassifiable mac} ->
-  clen:u64{let len = U64.v clen in len = length m /\ len = length c}  ->
-  n:uint8_p{length n = crypto_secretbox_NONCEBYTES} ->
-  k:uint8_p{length k = crypto_secretbox_KEYBYTES} ->
-  Stack u32
-    (requires (fun h -> live h m /\ live h c /\ live h mac /\ live h n /\ live h k))
-    (ensures  (fun h0 z h1 -> modifies_1 m h0 h1 /\ live h1 m))
-let crypto_secretbox_open_detached m c mac clen n k = Hacl.SecretBox.ZeroPad.crypto_secretbox_open_detached m c mac clen n k
 
-val crypto_secretbox_easy:
-  c:uint8_p ->
-  m:uint8_p ->
-  mlen:u64{let len = U64.v mlen in len <= length m /\ len + crypto_secretbox_MACBYTES <= length c}  ->
-  n:uint8_p{length n = crypto_secretbox_NONCEBYTES} ->
-  k:uint8_p{length k = crypto_secretbox_KEYBYTES} ->
-  Stack u32
-    (requires (fun h -> live h c /\ live h m /\ live h n /\ live h k))
-    (ensures  (fun h0 z h1 -> modifies_1 c h0 h1 /\ live h1 c))
-let crypto_secretbox_easy c m mlen n k =
-    Hacl.SecretBox.ZeroPad.crypto_secretbox_easy c m mlen n k
-
-val crypto_secretbox_open_easy:
-  m:uint8_p ->
-  c:uint8_p ->
-  clen:u64{let len = U64.v clen in len = length m + crypto_secretbox_MACBYTES /\ len = length c}  ->
-  n:uint8_p{length n = crypto_secretbox_NONCEBYTES} ->
-  k:uint8_p{length k = crypto_secretbox_KEYBYTES} ->
-  Stack u32
-    (requires (fun h -> live h c /\ live h m /\ live h n /\ live h k))
-    (ensures  (fun h0 z h1 -> modifies_1 m h0 h1 /\ live h1 m))
-let crypto_secretbox_open_easy m c clen n k =
-    Hacl.SecretBox.ZeroPad.crypto_secretbox_open_easy m c clen n k
+#reset-options "--initial_fuel 0 --max_fuel 0 --z3rlimit 20"
 
 val crypto_box_beforenm:
   k:uint8_p{length k = crypto_box_PUBLICKEYBYTES} ->
@@ -77,7 +40,19 @@ val crypto_box_beforenm:
     (requires (fun h -> live h k /\ live h pk /\ live h sk))
     (ensures  (fun h0 _ h1 -> modifies_1 k h0 h1))
 let crypto_box_beforenm k pk sk =
-  Hacl.Box.ZeroPad.crypto_box_beforenm k pk sk
+  push_frame();
+  let h0 = ST.get() in
+  let tmp = create (Hacl.Cast.uint8_to_sint8 0uy) 48ul in
+  let hsalsa_k = sub tmp 0ul 32ul in
+  let hsalsa_n = sub tmp 32ul 16ul in
+  (* Compute shared key *)
+  Curve25519.crypto_scalarmult hsalsa_k sk pk;
+  Hacl.Symmetric.HSalsa20.crypto_core_hsalsa20 k hsalsa_n hsalsa_k;
+  pop_frame();
+  0ul
+
+
+#reset-options "--initial_fuel 0 --max_fuel 0 --z3rlimit 10"
 
 val crypto_box_detached_afternm:
   c:uint8_p ->
@@ -90,7 +65,19 @@ val crypto_box_detached_afternm:
     (requires (fun h -> live h c /\ live h mac /\ live h m /\ live h n /\ live h k))
     (ensures  (fun h0 z h1 -> modifies_2 c mac h0 h1 /\ live h1 c /\ live h1 mac))
 let crypto_box_detached_afternm c mac m mlen n k =
-  Hacl.Box.ZeroPad.crypto_box_detached_afternm c mac m mlen n k
+  crypto_secretbox_detached c mac m mlen n k
+
+
+#reset-options "--initial_fuel 0 --max_fuel 0 --z3rlimit 20"
+
+let lemma_modifies_3_2 (c:uint8_p) (mac:uint8_p) h0 h1 h2 : Lemma
+  (requires (live h0 c /\ live h0 mac /\ live h1 mac /\ live h1 c /\ live h2 c /\ live h2 mac
+    /\ modifies_0 h0 h1 /\ modifies_2 c mac h1 h2))
+  (ensures  (modifies_3_2 c mac h0 h2))
+  = lemma_reveal_modifies_0 h0 h1; lemma_reveal_modifies_2 c mac h1 h2; lemma_intro_modifies_3_2 c mac h0 h2
+
+
+#reset-options "--initial_fuel 0 --max_fuel 0 --z3rlimit 20"
 
 val crypto_box_detached:
   c:uint8_p ->
@@ -104,7 +91,29 @@ val crypto_box_detached:
     (requires (fun h -> live h c /\ live h mac /\ live h m /\ live h n /\ live h pk /\ live h sk))
     (ensures  (fun h0 z h1 -> modifies_2 c mac h0 h1 /\ live h1 c /\ live h1 mac))
 let crypto_box_detached c mac m mlen n pk sk =
-  Hacl.Box.ZeroPad.crypto_box_detached c mac m mlen n pk sk 
+  push_frame();
+  let h0 = ST.get() in
+  let key = create (Hacl.Cast.uint8_to_sint8 0uy) 80ul in
+  let h0' = ST.get() in
+  let k = sub key 0ul 32ul in
+  let subkey = sub key 32ul 32ul in
+  let hsalsa_n = sub key 64ul 16ul in
+  (* Compute shared key *)
+  Curve25519.crypto_scalarmult k sk pk;
+  let h1 = ST.get() in
+  cut (modifies_0 h0 h1);
+  Hacl.Symmetric.HSalsa20.crypto_core_hsalsa20 subkey hsalsa_n k;
+  let h2 = ST.get() in
+  cut (modifies_0 h0 h2);
+  let z = crypto_secretbox_detached c mac m mlen n subkey in
+  let h3 = ST.get() in
+  cut (modifies_2 c mac h2 h3);
+  lemma_modifies_3_2 c mac h0 h2 h3;
+  pop_frame();
+  z
+
+
+#reset-options "--initial_fuel 0 --max_fuel 0 --z3rlimit 20"
 
 val crypto_box_open_detached:
   m:uint8_p ->
@@ -118,7 +127,20 @@ val crypto_box_open_detached:
     (requires (fun h -> live h c /\ live h mac /\ live h m /\ live h n /\ live h pk /\ live h sk))
     (ensures  (fun h0 z h1 -> modifies_1 m h0 h1 /\ live h1 m))
 let crypto_box_open_detached m c mac mlen n pk sk =
-  Hacl.Box.ZeroPad.crypto_box_open_detached m c mac mlen n pk sk 
+  push_frame();
+  let key = create (Hacl.Cast.uint8_to_sint8 0uy) 80ul in
+  let k = sub key 0ul 32ul in
+  let subkey = sub key 32ul 32ul in
+  let hsalsa_n = sub key 64ul 16ul in
+  (* Compute shared key *)
+  Curve25519.crypto_scalarmult k sk pk;
+  Hacl.Symmetric.HSalsa20.crypto_core_hsalsa20 subkey hsalsa_n k;
+  let z = crypto_secretbox_open_detached m c mac mlen n subkey in
+  pop_frame();
+  z
+
+
+#reset-options "--initial_fuel 0 --max_fuel 0 --z3rlimit 40"
 
 val crypto_box_easy_afternm:
   c:uint8_p ->
@@ -130,7 +152,10 @@ val crypto_box_easy_afternm:
     (requires (fun h -> live h c /\ live h m /\ live h n /\ live h k))
     (ensures  (fun h0 z h1 -> modifies_1 c h0 h1 /\ live h1 c))
 let crypto_box_easy_afternm c m mlen n k =
-  Hacl.Box.ZeroPad.crypto_box_easy_afternm c m mlen n k
+  let mlen' = Int.Cast.uint64_to_uint32 mlen in
+  Math.Lemmas.modulo_lemma (U64.v mlen) (pow2 32);
+  crypto_box_detached_afternm (sub c 16ul mlen') (sub c 0ul 16ul) (sub m 0ul mlen') mlen n k
+
 
 val crypto_box_easy:
   c:uint8_p ->
@@ -143,7 +168,16 @@ val crypto_box_easy:
     (requires (fun h -> live h c /\ live h m /\ live h n /\ live h pk /\ live h sk))
     (ensures  (fun h0 z h1 -> modifies_1 c h0 h1 /\ live h1 c))
 let crypto_box_easy c m mlen n pk sk =
-  Hacl.Box.ZeroPad.crypto_box_easy c m mlen n pk sk 
+  push_frame ();  
+  let mlen' = Int.Cast.uint64_to_uint32 mlen in
+  Math.Lemmas.modulo_lemma (U64.v mlen) (pow2 32);
+  let cmac   = create (uint8_to_sint8 0uy) 16ul in
+  let res = crypto_box_detached c cmac m mlen n pk sk in
+  blit cmac 0ul c 16ul 16ul;
+  pop_frame();
+  res
+
+
 
 val crypto_box_open_easy:
   m:uint8_p ->
@@ -156,7 +190,12 @@ val crypto_box_open_easy:
     (requires (fun h -> live h c /\ live h m /\ live h n /\ live h pk /\ live h sk))
     (ensures  (fun h0 z h1 -> modifies_1 m h0 h1 /\ live h1 m))
 let crypto_box_open_easy m c mlen n pk sk =
-  Hacl.Box.ZeroPad.crypto_box_open_easy m c mlen n pk sk 
+  let mlen' = Int.Cast.uint64_to_uint32 mlen in
+  Math.Lemmas.modulo_lemma (U64.v mlen) (pow2 32);
+  let mac = sub c 16ul 16ul in
+  assume (Hacl.Policies.declassifiable mac);
+  crypto_box_open_detached m c mac (U64.(mlen -^ 16uL)) n pk sk
+
 
 val crypto_box_open_detached_afternm:
   m:uint8_p ->
@@ -169,7 +208,7 @@ val crypto_box_open_detached_afternm:
     (requires (fun h -> live h c /\ live h mac /\ live h m /\ live h n /\ live h k))
     (ensures  (fun h0 z h1 -> modifies_1 m h0 h1 /\ live h1 m))
 let crypto_box_open_detached_afternm m c mac mlen n k =
-  Hacl.Box.ZeroPad.crypto_box_open_detached_afternm m c mac mlen n k
+  crypto_secretbox_open_detached m c mac mlen n k
 
 
 val crypto_box_open_easy_afternm:
@@ -182,4 +221,9 @@ val crypto_box_open_easy_afternm:
     (requires (fun h -> live h c /\ live h m /\ live h n /\ live h k))
     (ensures  (fun h0 z h1 -> modifies_1 m h0 h1 /\ live h1 c /\ live h1 k))
 let crypto_box_open_easy_afternm m c mlen n k =
-  Hacl.Box.ZeroPad.crypto_box_open_easy_afternm m c mlen n k 
+  let mlen' = Int.Cast.uint64_to_uint32 mlen in
+  Math.Lemmas.modulo_lemma (U64.v mlen) (pow2 32);
+  let mac = sub c 0ul 16ul in
+  assume (Hacl.Policies.declassifiable mac);
+  let c = sub c 16ul (U32.(mlen' -^ 16ul)) in
+  crypto_box_open_detached_afternm m c mac (U64.(mlen -^ 16uL)) n k
